<font color=white>  

John Beautz  
jpb375  

#MATH 3360 Homework 10

###Exercise 17A-7
$$1$$
This is the unit of itself
$$2$$
This is the unit of itself
$$x$$
This is a unit with itself
$$2x$$
This is a unit with itself
$$x+1$$
This is a zero divisor with $x+2$
$$x+2$$
This is a zero divisor with $x+1$
$$2x+1$$
This is a zero divisor with $2x+2$
$$2x+2$$
This is a zero divisor with $2x+1$
$$x^2$$
This is a unit of itself
$$x^2+1$$
This is a unit of itself
$$x^2+2$$
This is zero modulo
Each element is distinct modulo $x^2+1$ so this is a CSR.  


###Exercise 14A-10(ii)
$$x^5$$
$$x^5+x^4+x+1$$
$$x^4(x+1)+x+1$$
$$(x^4+1)(x+1)$$
$$(-x)(x+1)$$
$$x^2+x$$

###Exercise 14A-14(iii)
$$x^9 f(x) \cong 1 (mod x^2 + 2)$$
The GCD of $x^9$ and $x^2+2$ is $1$ in $\mathbb{Q}[x]$.
Therefore, there exists $g(x)$ such that
$$x^9f(x)+g(x)(x^2+2)=1$$
Use EEA to find these functions.  
$$\pmatrix{1  & 0             & x^9\\0  & 1             & x^2 + 2}$$

$$\pmatrix{1  & -x^7          & -2x^7\\0  & 1             & x^2 + 2}$$

$$\pmatrix{1  & -x^7+2x^5     & 4x^5\\0  & 1             & x^2 + 2}$$

$$\pmatrix{1  & -x^7+2x^5-4x^3& -8x^3\\0  & 1             & x^2+2}$$

$$\pmatrix{1  & -x^7+2x^5-4x^3+8x & 16x\\0  & 1                 & x^2+2}$$

$$\pmatrix{1      & -x^7+2x^5-4x^3+8x       & 16x\\-1/16x & 1+1/16x(x^7+2x^5-4x^3+8x)  & 2}$$

$$\pmatrix{1+1/2x^2 & -x^7+2x^5-4x^3+8x-8x(1+1/16x(x^7+2x^5-4x^3+8x)) & 0\\-1/32x & 1/2+1/32x(x^7+2x^5-4x^3+8x)  & 1}$$

Thus,
$$f(x)=-{1\over 32} x$$

###Exercise 17B-19(ii)
First, need to confirm $(x^4+x^2+x,x^4+x^3+1)=1$.  
$$\pmatrix{1  & 0     & x^4+x^3+1\\0  & 1     & x^4+x^2+x}$$

$$\pmatrix{1  & -1     & x^3-x^2-x+1\\0  & 1      & x^4+x^2+x}$$

$$\pmatrix{1  & -1       & x^3-x^2-x+1\\-x  & 1+x     & x^3}$$

$$\pmatrix{1  & -1         & x^3-x^2-x+1\\-1-x  & x       & x^2+x-1}$$

$$\pmatrix{1+x+x^2  & x^2+1       & 1\\-1-x     & x           & x^2+x-1}$$

So now, $(1+x+x^2)(x^4+x^3+1)+(x^2+1)(x^4+x^2+x)=1$.  

###Exercise 17C-25
Find a polynomial f (x) of degree ≤ 2 so that f (−1) = 1, f (0) = 0, f (1) = 2.

The auxiliary polynomial is
$$m(x)=(x+1)(x-1)x = x^3 - x$$
$$m'(x)=3x^2 - 1$$
Note, $m'(-1)=2$, $m'(0)=-1$, $m'(1)=2$.  
So,
$$e_1(x)={1\over 2}(x-1)x$$
$$e_2(x)=-(x-1)(x+1)$$
$$e_3(x)={1\over 2}(x+1)x$$

So finally,
$$f(x)=e_1(x)+2e_3(x)$$
$$f(x)={1\over 2}(x-1)x + (x+1)x$$



***THE END***
